pulse/examples/dsls/mini_steel/Pulse.Steel.Wrapper.fst
@@ -208,6 +208,7 @@ let read_atomic r #n #p =
 let write_atomic r x #n = fun _ ->
   R.atomic_write_u32 #_ #n r x
 
+let elim_pure_explicit p = fun _ -> elim_pure p
 let elim_pure _ #p = fun _ -> elim_pure p
 
 let intro_pure p _ = fun _ -> intro_pure p
