pulse/examples/dsls/mini_steel/Pulse.Elaborate.fst
@@ -56,7 +56,7 @@ let rec elab_open_commute' (e:term)
     | Tm_Star e1 e2 ->
       elab_open_commute' e1 v n;
       elab_open_commute' e2 v n
-    | Tm_ExistsSL u t body
+    | Tm_ExistsSL u t body _
     | Tm_ForallSL u t body ->
       elab_open_commute' t v n;
       elab_open_commute' body v (n + 1)
@@ -117,7 +117,7 @@ let rec elab_close_commute' (e:term)
     | Tm_Star e1 e2 ->
       elab_close_commute' e1 v n;
       elab_close_commute' e2 v n
-    | Tm_ExistsSL _ t body
+    | Tm_ExistsSL _ t body _
     | Tm_ForallSL _ t body ->
       elab_close_commute' t v n;
       elab_close_commute' body v (n + 1)    
